iris/algebra/functions.v
@@ -86,16 +86,6 @@ Section cmra.
       rewrite ?discrete_fun_lookup_singleton ?discrete_fun_lookup_singleton_ne //.
     by apply ucmra_unit_validN.
   Qed.
-  Lemma discrete_fun_singleton_valid x (y : B x) : ✓ discrete_fun_singleton x y ↔ ✓ y.
-  Proof.
-    by rewrite !cmra_valid_validN; setoid_rewrite discrete_fun_singleton_validN.
-  Qed.
-
-  Lemma discrete_fun_singleton_unit x : discrete_fun_singleton x (ε : B x) ≡ ε.
-  Proof.
-    move=>x'; destruct (decide (x = x')) as [->|];
-      by rewrite ?discrete_fun_lookup_singleton ?discrete_fun_lookup_singleton_ne.
-  Qed.
 
   Lemma discrete_fun_singleton_core x (y : B x) :
     core (discrete_fun_singleton x y) ≡ discrete_fun_singleton x (core y).
@@ -170,24 +160,5 @@ Section cmra.
   Proof.
     rewrite !cmra_update_updateP;
       eauto using discrete_fun_singleton_updateP_empty with subst.
-  Qed.
-
-  Lemma discrete_fun_updateP `{!Finite A} f P Q :
-    (∀ a, f a ~~>: P a) → (∀ f', (∀ a, P a (f' a)) → Q f') → f ~~>: Q.
-  Proof.
-    repeat setoid_rewrite cmra_total_updateP. intros Hf HP n h Hh.
-    destruct (finite_choice
-      (λ a y, P a y ∧ ✓{n} (y ⋅ (h a)))) as [f' Hf']; first naive_solver.
-    naive_solver.
-  Qed.
-  Lemma discrete_fun_updateP' `{!Finite A} f P :
-    (∀ a, f a ~~>: P a) → f ~~>: λ f', ∀ a, P a (f' a).
-  Proof. eauto using discrete_fun_updateP. Qed.
-
-  Lemma discrete_fun_update f g :
-    (∀ a, f a ~~> g a) → f ~~> g.
-  Proof.
-    repeat setoid_rewrite cmra_total_update.
-    intros Hfg n h Hh a. apply (Hfg a), Hh.
   Qed.
 End cmra.
