iris_deprecated/base_logic/auth.v
@@ -11,9 +11,10 @@ Import uPred.
 
 (* The CMRA we need. *)
 Class authG Σ (A : ucmra) := AuthG {
-  #[local] auth_inG :: inG Σ (authR A);
+  auth_inG : inG Σ (authR A);
   #[global] auth_cmra_discrete :: CmraDiscrete A;
 }.
+Local Existing Instance auth_inG.
 
 Definition authΣ (A : ucmra) : gFunctors := #[ GFunctor (authR A) ].
 
