iris_heap_lang/derived_laws.v
@@ -81,13 +81,13 @@ Proof.
   iDestruct (array_app with "Hl") as "[Hl1 Hl]".
   iDestruct (array_cons with "Hl") as "[Hl2 Hl3]".
   assert (off < length vs) as H by (apply lookup_lt_is_Some; by eexists).
-  rewrite length_take min_l; last by lia. iFrame "Hl2".
+  rewrite take_length min_l; last by lia. iFrame "Hl2".
   iIntros (w) "Hl2".
   clear Hlookup. assert (<[off:=w]> vs !! off = Some w) as Hlookup.
   { apply list_lookup_insert. lia. }
   rewrite -[in (l ↦∗{_} <[off:=w]> vs)%I](take_drop_middle (<[off:=w]> vs) off w Hlookup).
   iApply array_app. rewrite take_insert; last by lia. iFrame.
-  iApply array_cons. rewrite length_take min_l; last by lia. iFrame.
+  iApply array_cons. rewrite take_length min_l; last by lia. iFrame.
   rewrite drop_insert_gt; last by lia. done.
 Qed.
 
@@ -96,7 +96,7 @@ Lemma pointsto_seq_array l dq v n :
   ([∗ list] i ∈ seq 0 n, (l +ₗ (i : nat)) ↦{dq} v) -∗
   l ↦∗{dq} replicate n v.
 Proof.
-  rewrite /array. iInduction n as [|n' IH] forall (l); simpl.
+  rewrite /array. iInduction n as [|n'] "IH" forall (l); simpl.
   { done. }
   iIntros "[$ Hl]". rewrite -fmap_S_seq big_sepL_fmap.
   setoid_rewrite Nat2Z.inj_succ. setoid_rewrite <-Z.add_1_l.
