iris_heap_lang/lib/array.v
@@ -57,7 +57,7 @@ Section proof.
     [[{ l ↦∗ vs }]] array_free #l #n @ s; E [[{ RET #(); True }]].
   Proof.
     iIntros (Hlen Φ) "Hl HΦ".
-    iInduction vs as [|v vs IH] forall (l n Hlen); subst n; wp_rec; wp_pures.
+    iInduction vs as [|v vs] "IH" forall (l n Hlen); subst n; wp_rec; wp_pures.
     { iApply "HΦ". done. }
     iDestruct (array_cons with "Hl") as "[Hv Hl]".
     wp_free. wp_pures. iApply ("IH" with "[] Hl"); eauto with lia.
@@ -77,7 +77,7 @@ Section proof.
     [[{ RET #(); dst ↦∗ vsrc ∗ src ↦∗{dq} vsrc }]].
   Proof.
     iIntros (Hvdst Hvsrc Φ) "[Hdst Hsrc] HΦ".
-    iInduction vdst as [|v1 vdst IH] forall (n dst src vsrc Hvdst Hvsrc);
+    iInduction vdst as [|v1 vdst] "IH" forall (n dst src vsrc Hvdst Hvsrc);
       destruct vsrc as [|v2 vsrc]; simplify_eq/=; try lia; wp_rec; wp_pures.
     { iApply "HΦ". auto with iFrame. }
     iDestruct (array_cons with "Hdst") as "[Hv1 Hdst]".
@@ -107,7 +107,7 @@ Section proof.
     wp_lam.
     wp_alloc dst as "Hdst"; first by auto.
     wp_smart_apply (twp_array_copy_to with "[$Hdst $Hvl]") as "[Hdst Hl]".
-    - rewrite length_replicate Z2Nat.id; lia.
+    - rewrite replicate_length Z2Nat.id; lia.
     - auto.
     - wp_pures.
       iApply "HΦ"; by iFrame.
@@ -139,7 +139,7 @@ Section proof.
       }}}.
     Proof.
       iIntros (Hn Φ) "[Hl Hf] HΦ".
-      iInduction k as [|k IH] forall (i Hn); simplify_eq/=; wp_rec; wp_pures.
+      iInduction k as [|k] "IH" forall (i Hn); simplify_eq/=; wp_rec; wp_pures.
       { rewrite bool_decide_eq_true_2; last (repeat f_equal; lia).
         wp_pures. iApply ("HΦ" $! []). auto. }
       rewrite bool_decide_eq_false_2; last naive_solver lia.
@@ -166,7 +166,7 @@ Section proof.
       }]].
     Proof.
       iIntros (Hn Φ) "[Hl Hf] HΦ".
-      iInduction k as [|k IH] forall (i Hn); simplify_eq/=; wp_rec; wp_pures.
+      iInduction k as [|k] "IH" forall (i Hn); simplify_eq/=; wp_rec; wp_pures.
       { rewrite bool_decide_eq_true_2; last (repeat f_equal; lia).
         wp_pures. iApply ("HΦ" $! []). auto. }
       rewrite bool_decide_eq_false_2; last naive_solver lia.
@@ -232,7 +232,7 @@ Section proof.
       ([∗ list] k↦v ∈ vs, ∃ x, ⌜v = g x⌝ ∗ Q k x) -∗
       ∃ xs, ⌜ vs = g <$> xs ⌝ ∗ [∗ list] k↦x ∈ xs, Q k x.
     Proof.
-      iIntros "Hvs". iInduction vs as [|v vs IH] forall (Q); simpl.
+      iIntros "Hvs". iInduction vs as [|v vs] "IH" forall (Q); simpl.
       { iExists []. by auto. }
       iDestruct "Hvs" as "[(%x & -> & Hv) Hvs]".
       iDestruct ("IH" with "Hvs") as (xs ->) "Hxs".
@@ -253,7 +253,7 @@ Section proof.
       iIntros (Hn Φ) "Hf HΦ". iApply (wp_array_init with "Hf"); first done.
       iIntros "!>" (l vs). iDestruct 1 as (<-) "[Hl Hvs]".
       iDestruct (big_sepL_exists_eq with "Hvs") as (xs ->) "Hxs".
-      iApply "HΦ". iFrame "Hl Hxs". by rewrite length_fmap.
+      iApply "HΦ". iFrame "Hl Hxs". by rewrite fmap_length.
     Qed.
     Lemma twp_array_init_fmap stk E n f :
       (0 < n)%Z →
@@ -269,7 +269,7 @@ Section proof.
       iIntros (Hn Φ) "Hf HΦ". iApply (twp_array_init with "Hf"); first done.
       iIntros (l vs). iDestruct 1 as (<-) "[Hl Hvs]".
       iDestruct (big_sepL_exists_eq with "Hvs") as (xs ->) "Hxs".
-      iApply "HΦ". iFrame "Hl Hxs". by rewrite length_fmap.
+      iApply "HΦ". iFrame "Hl Hxs". by rewrite fmap_length.
     Qed.
   End array_init_fmap.
 End proof.
