iris_heap_lang/lib/ticket_lock.v
@@ -28,8 +28,8 @@ Local Definition release : val :=
 
 (** The CMRAs we need. *)
 Class tlockG Σ :=
-  #[local] tlock_G ::
-    inG Σ (authR (prodUR (optionUR (exclR natO)) (gset_disjUR nat))).
+  tlock_G : inG Σ (authR (prodUR (optionUR (exclR natO)) (gset_disjUR nat))).
+Local Existing Instance tlock_G.
 
 Definition tlockΣ : gFunctors :=
   #[ GFunctor (authR (prodUR (optionUR (exclR natO)) (gset_disjUR nat))) ].
